Initial parameterization pass.

lib/ArithSolver/ArithM.lean
@@ -6,13 +6,18 @@ import ArithSolver.Basic
 import ArithSolver.Int
 
 open Lean
+open Std (HashMap)
 
 namespace ArithSolver
 
-private def notExpr : Expr := mkConst ``Not
+namespace ArithTheory
+
+section ExpressionUtils
 
 def natExpr : Expr := mkConst ``Nat
 def intExpr := mkConst ``Int
+
+private def notExpr : Expr := mkConst ``Not
 
 def intAddConst : Expr :=
   let f := mkConst ``HAdd.hAdd [levelZero, levelZero, levelZero]
@@ -37,13 +42,17 @@ def intNegConst : Expr :=
 -- A structure used to denote an integer expression
 structure IntExpr where
   toExpr : Expr
-  deriving Inhabited
+  deriving BEq, Hashable, Inhabited
+
+namespace IntExpr
 
 instance : Coe IntExpr Expr where
   coe := IntExpr.toExpr
 
 instance : Add IntExpr where
   add := λx y => IntExpr.mk (mkAppN intAddConst #[x, y])
+
+end IntExpr
 
 -- Create a nat lit as an int
 def natLitAsIntExpr (n:Nat) : IntExpr :=
@@ -67,95 +76,211 @@ def mkIntNonNegExpr (e:Expr) : Expr := mkApp intNonNegExpr e
 private def intEqExpr : Expr := mkApp (mkConst ``Eq [levelOne]) (mkConst ``Int)
 def mkIntEq0Expr (e:Expr) : Expr := mkAppN intEqExpr #[e, intZeroExpr]
 
-namespace State
+end ExpressionUtils
+
+-- Represents a polynomial.
+structure Poly where
+  -- Poly should be a sorted array of non-zero integers and variable pairs.
+  -- The
+  elements : Array (Int × TheoryVar)
+  deriving BEq, Hashable, Repr
+
+namespace Poly
+
+-- | Create polynomial denoting constant zero.
+def zero : Poly := ⟨#[]⟩
+
+instance : Inhabited Poly := ⟨zero⟩
+
+-- | Create polynomial denoting constant zero.
+protected def one : Poly := ⟨#[(1, ⟨0⟩)]⟩
+
+-- | @add p i _ v@ returns poly denoting @p + i*v@.
+def add : ∀(p:Poly) (m:Int), TheoryVar → Poly
+| ⟨a⟩, q, v =>
+  let rec loop : ∀(i : Nat), Poly
+      | 0 => ⟨a.insertAt 0 (q, v)⟩
+      | Nat.succ i =>
+        let (p,u) := a[i]
+        if u < v then
+          ⟨a.insertAt (i+1) (q,v)⟩
+        else if v < u then
+          loop i
+        else -- v = u
+          let q := p+q
+          if q = 0 then
+            ⟨a.eraseIdx i⟩
+          else
+            ⟨a.set! i (q,v)⟩
+  loop a.size
+
+protected def toString : Poly → String
+| ⟨a⟩ =>
+  let scalarProd : Int × TheoryVar → String
+        | (m,v) => s!"{m}*{v}"
+  let firstScalarProd : Int × TheoryVar → String
+        | (m, ⟨0⟩) => toString m
+        | p => scalarProd p
+  let polyIns := λ(e:String) h => s!"{e} + {scalarProd h}"
+  a[1:].foldl polyIns (firstScalarProd a[0])
+
+instance : ToString Poly where
+  toString := Poly.toString
+
+end Poly
+
+-- Definition associated with a variable.
+inductive Decl
+  -- Theory variable is equal to the expression.
+| uninterp : Var → Decl
+  -- Theory variable is equal to polynomial.
+| poly : Poly → Decl
+deriving BEq, Hashable
+
+namespace Decl
+
+protected def toString : Decl → String
+| uninterp v => s!"uninterp {v}"
+| poly p => s!"poly {p}"
+
+instance : ToString Decl where
+  toString := Decl.toString
+
+instance : Inhabited Decl := ⟨uninterp arbitrary⟩
+
+end Decl
+
+-- | An atomic predicate
+inductive Pred where
+-- This denotes a proof of the form (v = 0)
+| IsEq0 : TheoryVar → Pred
+-- This denotes a proof of the form (Not (v = 0))
+| IsNe0 : TheoryVar → Pred
+-- This denotes a proof of the form (Int.NonNeg v)
+| IsGe0 : TheoryVar → Pred
+  deriving Inhabited
+
+namespace Pred
+
+protected def toString : Pred → String
+| IsEq0 v => s!"IsEq0 {v}"
+| IsNe0 v => s!"IsNe0 {v}"
+| IsGe0 v => s!"IsGe0 {v}"
+
+instance : ToString Pred := ⟨Pred.toString⟩
+
+end Pred
+
+def oneVar : TheoryVar := ⟨0⟩
+
+structure State : Type where
+  exprMap : HashMap Decl TheoryVar := Std.mkHashMap.insert (Decl.poly Poly.one) oneVar
+  vars : Array Decl := #[Decl.poly Poly.one]
+  preds : Array Pred := #[]
 
 mutual
 
-partial def scalarProd (s:State) : Int × Var → IntExpr
+variable (r:IO.Ref State)
+variable (f: Var → IO IntExpr)
+
+partial def scalarProd : Int × TheoryVar → IO IntExpr
 | (m, ⟨0⟩) => m
-| (m,  v) => IntExpr.mk (mkAppN intMulConst #[m, s.varExpr v])
+| (m,  v) => do IntExpr.mk (mkAppN intMulConst #[m, ← thvarExpr v])
 
 -- | Map polynomial to expression given mapping from variables
 -- to expressions.
 -- The optional parameter allowss this to to only take the first n elements.
-partial def polyExpr (s:State) (poly:Poly) (limit: optParam Nat (poly.elements.size)): IntExpr :=
+partial def polyExpr (poly:Poly) (limit: optParam Nat (poly.elements.size)) : IO IntExpr := do
+  if limit > poly.elements.size then
+    panic! "polyExpr given bad limit."
   if limit = 0 then
     (0 : Int)
-  else Id.run do
-    let mut e := scalarProd s poly.elements[0]
+  else do
+    let mut e ← scalarProd poly.elements[0]
     for p in poly.elements[1:limit] do
-      e := e + scalarProd s p
+      e := e + (← scalarProd p)
     pure e
 
-partial def varExpr (s:State) (v:Var) : IntExpr :=
-  match s.varExprs.get! v.index.toNat with
-  | Decl.uninterp e => IntExpr.mk e
-  | Decl.poly p => polyExpr s p
+-- | Return Lean expression associated with IntExpr
+partial def thvarExpr (v:TheoryVar) : IO IntExpr := do
+  let s ← r.get
+  if p : v.toNat < s.vars.size then
+    match s.vars.get ⟨v.toNat, p⟩  with
+    | Decl.uninterp v => do
+      f v
+    | Decl.poly p => polyExpr p
+  else
+    panic! s!"Invalid theory variable index {v} (max = {s.vars.size})"
 
 end
 
-def predExpr (s:State) : Pred → Expr
-| Pred.IsEq0 v => mkIntEq0Expr (s.varExpr v)
-| Pred.IsNe0 v => mkApp notExpr (mkIntEq0Expr (s.varExpr v))
-| Pred.IsGe0 v => mkIntNonNegExpr (s.varExpr v)
-
--- | Add assertions to local context.
--- Return new local context along with array of free variables identifying assertions.
-def addAssertions (s : State) (lctx:LocalContext) : MetaM (LocalContext × Array Expr) := do
-  let mut lctx := lctx
-  let mut fvars : Array Expr := #[]
-  for a in s.assertions do
-    let newVar ← mkFreshFVarId
-    fvars := fvars.push (mkFVar newVar)
-    match a.origin with
-    | some prevVar =>
-      -- FIXME: Make sure erasing the previous declaration does not break things.
-      lctx := lctx.erase prevVar
-    | none =>
-      pure ()
-    lctx := lctx.mkLocalDecl newVar a.name (s.predExpr a.prop)
-  pure (lctx, fvars)
-
-end State
-
-abbrev ArithM  := StateRefT State MetaM
-
-@[inline] def ArithM.run (m : ArithM α) (s : State := {}) : MetaM (α × State) :=
-  StateRefT'.run m s
+abbrev ArithM := ReaderT (IO.Ref State) SolverM
 
 -- | Return a theory variable associated with the given uninterpreted Lean expression.
-private def getDeclVar (d:Decl) : ArithM Var := do
-  let s ← get
+private def getVar (d:Decl) : ArithM TheoryVar := do
+  let r ← read
+  let s ← r.get
   match s.exprMap.find? d with
   | none => pure ()
   | some v => return v
-  let newVar := ⟨OfNat.ofNat s.varExprs.size⟩
-  IO.println s!"New variable: {newVar} := {d}"
-  let newExprMap  := s.exprMap.insert d newVar
-  let newVarExprs := s.varExprs.push d
-  if (OfNat.ofNat s.varExprs.size : UInt32) = 0 then
+  let newVar := ⟨OfNat.ofNat s.vars.size⟩
+  if (newVar.index : UInt32) = 0 then
     throwError m!"Only 2^32 arithmetic variables allowed."
-  set { s with exprMap := newExprMap, varExprs := newVarExprs }
+  r.set
+    { s with exprMap := s.exprMap.insert d newVar,
+             vars := s.vars.push d }
   return newVar
 
 -- | Return a theory variable associated with the given uninterpreted Lean expression.
-def getUninterpVar (e:Expr) : ArithM Var := getDeclVar (Decl.uninterp e)
+def getUninterpVar (v:Var) : ArithM TheoryVar := getVar (Decl.uninterp v)
 
 -- | Return a theory variable associated with the given uninterpreted Lean expression.
-def getPolyVar (p:Poly) : ArithM Var := getDeclVar (Decl.poly p)
+def getPolyVar (p:Poly) : ArithM TheoryVar := getVar (Decl.poly p)
 
+
+/-
 -- | Assert a predicate holds using the given expression to refer to the
 -- proof.
-def assertPred (origin:Option FVarId) (userName:Name) (proof:Expr) (prop:Pred) : ArithM Unit := do
+def assertPred (origin:Option FVarId) (userName:Name) (proof:Expr) (prop:Pred) : ArithM Solver Unit := do
   let a := { origin := origin, name := userName, proof := proof, prop := prop }
   modifyGet fun s => ((), { s with assertions := s.assertions.push a })
+-/
 
-def varExpr (v:Var) : ArithM IntExpr := do
-  let s ← get
-  pure $ s.varExpr v
+def getThvarExpr (v:TheoryVar) : ArithM IntExpr := do
+  let svc ← (read : SolverM _)
+  let f (v:Var) : IO IntExpr := IntExpr.mk <$> svc.varExpr v
+  let r ← read
+  thvarExpr r f v
 
-def polyExpr (poly:Poly) : ArithM IntExpr := do
-  let s ← get
-  pure $ s.polyExpr poly
+-- | Return expression associated with in solver.
+def getPolyExpr (poly:Poly) : ArithM IntExpr := do
+  let svc ← (read : SolverM _)
+  let f (v:Var) : IO IntExpr := IntExpr.mk <$> svc.varExpr v
+  let r ← read
+  polyExpr r f poly
+
+def getTheoryPred (p:Pred) : ArithM TheoryPred := do
+  let r ← read
+  let s ← r.get
+  if TheoryPred.max ≤ s.preds.size then
+    throwError "Only 2^32 arithmetic variables allowed."
+  let n := TheoryPred.ofNat (s.preds.size)
+  r.set { s with preds := s.preds.push p }
+  pure n
+
+def mthvarExpr (r: IO.Ref State) (f : Var → IO Expr)  (thv : TheoryVar) : IO Expr := do
+  IntExpr.toExpr <$> thvarExpr r (fun v => IntExpr.mk <$> f v) thv
+
+def predExpr (r : IO.Ref State) (f : Var → IO Expr) (idx : TheoryPred) : IO Expr := do
+  let s ← r.get
+  if lt : idx.toNat < s.preds.size  then
+    match s.preds.get ⟨idx.toNat, lt⟩  with
+    | Pred.IsEq0 v => mkIntEq0Expr <$> mthvarExpr r f v
+    | Pred.IsNe0 v => mkApp notExpr <$> (mkIntEq0Expr <$> mthvarExpr r f v)
+    | Pred.IsGe0 v => mkIntNonNegExpr <$> mthvarExpr r f v
+  else
+    panic s!"Invalid predicate index {idx} (max = {s.preds.size})"
+
+end ArithTheory
 
 end ArithSolver
