lib/ArithSolver/ConstantTheory.lean
@@ -1,0 +1,46 @@
+import ArithSolver.Basic
+
+open Lean
+open Std(HashMap)
+
+namespace ArithSolver
+
+namespace ConstantTheory
+
+structure State where
+  -- Maps expressions to theory variable and cached refl proof.
+  exprMap : HashMap Expr (TheoryVar × Expr) := Std.mkHashMap
+  values : Array Expr := #[]
+
+def exprVar (r:IO.Ref State) (e:Expr) : MetaM (ExprEvalResult TheoryVar) := do
+  let s ← r.get
+  match s.exprMap.find? e with
+  | none => pure ()
+  | some (v,pr) =>
+    return { var := v, varExpr := e , eq := pr }
+  let v := TheoryVar.ofNat s.values.size
+  let tp ← Meta.inferType e
+  let lvl : Level ←
+        match ← Meta.inferType tp with
+        | Expr.sort lvl .. => pure lvl
+        | utp => throwError s!"Could not determine level of {utp}"
+  let pr : Expr := mkAppN (mkConst `rfl [lvl]) #[tp, e]
+  r.set { exprMap := s.exprMap.insert e (v, pr), values := s.values.push e }
+  return { var := v, varExpr := e, eq := pr }
+
+def varExpr (r:IO.Ref State) (f : Var → IO Expr) (v:TheoryVar) : IO Expr := do
+  pure (←r.get).values[v.toNat]
+
+def predExpr (f : Var → IO Expr) (p:TheoryPred) : IO Expr :=
+  panic! "Constant theory has no predicates."
+
+
+def ops (r:IO.Ref State) : TheoryOps :=
+  { varExpr := varExpr r,
+    predExpr := predExpr,
+    exprVar := fun e => exprVar r e
+    }
+
+end ConstantTheory
+
+end ArithSolver
