lib/ArithSolver/IntNormalization.lean
@@ -8,8 +8,10 @@ open Lean
 open Lean.Meta
 
 namespace ArithSolver
-namespace State
 
+namespace ArithTheory
+
+section Lemmas
 private
 theorem sum0Lemma (p q v:Int) : p*v + q*v = (p+q)*v := Eq.symm (Int.add_mul _ _ _)
 
@@ -39,15 +41,17 @@ theorem polyProofAddContextLemma {x c a:Int} (h:x + c = a) (y:Int)
   : (x + y) + c = a + y := by
   simp [h.symm, Int.add_assoc, Int.add_comm y c]
 
+end Lemmas
+
 -- polyProofAddContext s x c a h poly idx where h is a proof of "x + c = a" returns
 -- a proof "(x + poly[idx] + poly[idx+1] + ..) + c = a + poly[idx] + poly[idx+1] + .."
 private
-def polyProofAddContext (s:State) (x c a:IntExpr) (h:Expr) (poly:Poly) (idx:Nat) : Expr := Id.run do
+def polyProofAddContext (ref:IO.Ref State) (f:Var → IO IntExpr) (x c a:IntExpr) (h:Expr) (poly:Poly) (idx:Nat) : IO Expr := do
   let mut x := x
   let mut a := a
   let mut h := h
   for p in poly.elements[idx:] do
-    let y := s.scalarProd p
+    let y ← scalarProd ref f p
     h := mkAppN (mkConst ``polyProofAddContextLemma) #[x, c, a, h, y]
     x := x + y
     a := a + y
@@ -56,66 +60,66 @@ def polyProofAddContext (s:State) (x c a:IntExpr) (h:Expr) (poly:Poly) (idx:Nat)
 -- | @addProof f p m v@ returns proof showing that
 -- @p.expr + firstScalarProd f (m, v) = (p.add m v).expr@.
 private
-def polyAddProof (s:State) : ∀(poly:Poly) (q:Int), q ≠ 0 → Var → Expr
-| poly, q, g, v =>
-  let c := s.scalarProd (q,v)
-  let rec loop : ∀(i : Nat), Expr
-      | 0 =>
+def polyAddProof (ref:IO.Ref State) (f:Var → IO IntExpr) : ∀(poly:Poly) (q:Int), q ≠ 0 → TheoryVar → IO Expr
+| poly, q, g, v => do
+  let c ← scalarProd ref f (q,v)
+  let rec loop : ∀(i : Nat), IO Expr
+      | 0 => do
         if poly.elements.size = 0 then
           -- Prove (0:Int) + firstScalarProd f (q,v) = firstScalarProd f (q,v)
           mkApp (mkConst `Int.zero_add) c
-        else Id.run do
-          let x := s.scalarProd poly.elements[0]
+        else
+          let x ← scalarProd ref f poly.elements[0]
           let a := c + x
           let h := mkAppN (mkConst `Int.add_comm) #[x, c]
-          polyProofAddContext s x c a h poly 1
-      | Nat.succ i =>
+          polyProofAddContext ref f x c a h poly 1
+      | Nat.succ i => do
         let (p,u) := poly.elements[i]
         if u < v then
-          let x := s.polyExpr poly (limit := i+1)
+          let x ← polyExpr ref f poly (limit := i+1)
           let a := x + c
           let h := mkAppN (mkConst ``Eq.refl [levelOne]) #[intExpr, a]
-          polyProofAddContext s x c a h poly (i+1)
+          polyProofAddContext ref f x c a h poly (i+1)
         else if v < u then
           loop i
         else -- v = u
           if p+q = 0 then
             if i = 0 then
-              let x := s.scalarProd poly.elements[0]
+              let x ← scalarProd ref f poly.elements[0]
               let a := (0 : Int)
               let rflExpr := mkAppN (mkConst ``rfl [levelOne]) #[intExpr, intZeroExpr]
               -- Create proof: -q*v + q*v = 0.
-              let h := mkAppN (mkConst ``cancel0Lemma) #[ (-q : Int), q, rflExpr, s.varExpr v]
-              polyProofAddContext s x c a h poly (i+1)
+              let h := mkAppN (mkConst ``cancel0Lemma) #[ (-q : Int), q, rflExpr, ← thvarExpr ref f v]
+              polyProofAddContext ref f x c a h poly (i+1)
             else
-              let a := s.polyExpr poly i
-              let x := a + s.scalarProd poly.elements[i]
+              let a ← polyExpr ref f poly i
+              let x := a + (← scalarProd ref f poly.elements[i])
               let rflExpr := mkAppN (mkConst ``rfl [levelOne]) #[intExpr, intZeroExpr]
               -- Create proof: (r + -q*v) + q*v = r.
-              let h := mkAppN (mkConst ``cancelLemma) #[a, (-q : Int), q, s.varExpr v, rflExpr]
-              polyProofAddContext s x c a h poly (i+1)
+              let h := mkAppN (mkConst ``cancelLemma) #[a, (-q : Int), q, ← thvarExpr ref f v, rflExpr]
+              polyProofAddContext ref f x c a h poly (i+1)
           else
             if i = 0 then
-              let x := s.scalarProd poly.elements[0]
-              let a := s.scalarProd (p+q, v)
+              let x ← scalarProd ref f poly.elements[0]
+              let a ← scalarProd ref f (p+q, v)
               --  Create proof (p*v) + (q*v) = (p+q) * v
-              let h := mkAppN (mkConst ``sum0Lemma) #[p, q, s.varExpr v]
-              polyProofAddContext s x c a h poly (i+1)
+              let h := mkAppN (mkConst ``sum0Lemma) #[p, q, ← thvarExpr ref f v]
+              polyProofAddContext ref f x c a h poly (i+1)
             else
-              let r := s.polyExpr poly i
-              let x := r + s.scalarProd poly.elements[i]
-              let a := r + s.scalarProd (p+q, v)
-              let h := mkAppN (mkConst ``sumLemma) #[r, p, q, s.varExpr v]
-              polyProofAddContext s x c a h poly (i+1)
+              let r ← polyExpr ref f poly i
+              let x := r + (←scalarProd ref f poly.elements[i])
+              let a := r + (←scalarProd ref f (p+q, v))
+              let h := mkAppN (mkConst ``sumLemma) #[r, p, q, ←thvarExpr ref f v]
+              polyProofAddContext ref f x c a h poly (i+1)
   loop poly.elements.size
-
-end State
 
 -- @polyAddProof s poly q _ v@ returns a proof that
 --   @poly.expr varExpr s + firstScalarProd s.varExpr (m, v) = (poly.add m v).expr s.varExpr@.
-def polyAddProof (poly:Poly) (q:Int) (q_ne:q ≠ 0) (v:Var) : ArithM Expr := do
-  let s ← get
-  pure $ s.polyAddProof poly q q_ne v
+def getPolyAddProof (poly:Poly) (q:Int) (q_ne:q ≠ 0) (v:TheoryVar) : ArithM Expr := do
+  let svc ← (read : SolverM _)
+  let ref ← read
+  let f (v:Var) := IntExpr.mk <$> svc.varExpr v
+  polyAddProof ref f poly q q_ne v
 
 section Normalization
 
@@ -162,61 +166,75 @@ private theorem mul_rhs_poly_lemma {m x y a b:Int} (g: a + (m*y)*x = b) : a + m*
   rw [Int.mul_assoc, Int.mul_comm y x] at g
   exact g
 
+theorem uninterpVarLemma {e v a m b:Int} (eq:e = v) (pr:a + m * v = b) : a + m * e = b := by
+  rw [eq]
+  exact pr
+
+structure AddResult where
+  poly : Poly
+  polyExpr : Expr
+  equivProof : Expr
+
 -- | @appendAddExpr poly m e@ returns poly equivalent to `poly + m*e` along with proof that that
 -- poly.expr + m*e = ret.expr
 private
-partial def appendAddExprFromInt (m:Int) (m_ne:m ≠ 0) (e:Expr) (poly:Poly)
-   : ArithM (Poly × Expr) := do
-
+partial def appendAddExprFromInt (m:Int) (m_ne:m ≠ 0) (e:Expr) (poly:Poly) : ArithM AddResult := do
   match ← matchIntLit e with
   | none => pure ()
   | some x =>
     let r ←
       if x_ne : x = 0 then
-        let aexpr ← polyExpr poly
+        let aexpr ← getPolyExpr poly
         let pr := mkAppN (mkConst ``rfl [levelOne]) #[intExpr, aexpr]
-        pure (poly, pr)
+        pure {
+          poly := poly
+          polyExpr := ← getPolyExpr poly
+          equivProof := pr
+        }
       else
         let y := m * x
         -- pr: poly + m * x * 1 = r
-        let pr ← polyAddProof poly y (Int.mul_ne_zero m_ne x_ne) Var.one
-        return (poly.add y Var.one, pr)
+        let pr ← getPolyAddProof poly y (Int.mul_ne_zero m_ne x_ne) oneVar
+        let poly := poly.add y oneVar
+        return {
+          poly := poly,
+          polyExpr := ← getPolyExpr poly,
+          equivProof := pr
+        }
     return r
-
   -- Match addition
+  let aexpr ← getPolyExpr poly
   match ← matchBinOp intAddConst intExpr e with
   | none => pure ()
   | some (x, y) => do
-    let aexpr ← polyExpr poly
-    let (poly, x_pr) ← appendAddExprFromInt m m_ne x poly
-    let bexpr ← polyExpr poly
-    let (poly, y_pr) ← appendAddExprFromInt m m_ne y poly
-    let cexpr ← polyExpr poly
+    let { poly := poly, polyExpr := bexpr, equivProof := x_pr }
+          ← appendAddExprFromInt m m_ne x poly
+    let { poly := poly, polyExpr := cexpr, equivProof := y_pr }
+          ← appendAddExprFromInt m m_ne y poly
     let pr := mkAppN (mkConst ``add_poly_lemma) #[m, x, y, aexpr, bexpr, cexpr, x_pr, y_pr]
-    return (poly, pr)
+    return { poly := poly, polyExpr := ← getPolyExpr poly, equivProof := pr }
 
   -- Match sub
   match ← matchBinOp intSubConst intExpr e with
   | none => pure ()
   | some (x, y) => do
-    let aexpr ← polyExpr poly
-    let (poly, x_pr) ← appendAddExprFromInt m m_ne x poly
-    let bexpr ← polyExpr poly
-    let (poly, y_pr) ← appendAddExprFromInt (- m) (Int.neg_ne_zero m_ne) y poly
-    let cexpr ← polyExpr poly
+    let { poly := poly, polyExpr := bexpr, equivProof := x_pr }
+          ← appendAddExprFromInt m m_ne x poly
+    let bexpr ← getPolyExpr poly
+    let { poly := poly, polyExpr := cexpr, equivProof := y_pr }
+          ← appendAddExprFromInt (- m) (Int.neg_ne_zero m_ne) y poly
     let pr := mkAppN (mkConst ``sub_poly_lemma) #[m, x, y, aexpr, bexpr, cexpr, x_pr, y_pr]
-    return (poly, pr)
+    return { poly := poly, polyExpr := ← getPolyExpr poly, equivProof := pr }
 
   -- Match negation
   let negExpr := mkAppN (mkConst ``Neg.neg [levelZero]) #[intExpr, mkConst ``Int.instNegInt]
   match ← matchUnaryOp intNegConst intExpr e with
   | none => pure ()
   | some x => do
-    let aexpr ← polyExpr poly
-    let (poly, x_pr) ← appendAddExprFromInt (-m) (Int.neg_ne_zero m_ne) x poly
-    let bexpr ← polyExpr poly
+    let { poly := poly, polyExpr := bexpr, equivProof := x_pr }
+          ← appendAddExprFromInt (-m) (Int.neg_ne_zero m_ne) x poly
     let pr := mkAppN (mkConst ``neg_poly_lemma) #[m, x, aexpr, bexpr, x_pr]
-    return (poly, pr)
+    return { poly := poly, polyExpr := ← getPolyExpr poly, equivProof := pr }
 
   -- Match scalar multiplication
   match ← matchBinOp intMulConst intExpr e with
@@ -226,38 +244,44 @@ partial def appendAddExprFromInt (m:Int) (m_ne:m ≠ 0) (e:Expr) (poly:Poly)
     match ← matchIntLit x with
     | none => pure ()
     | some xn =>
-      let aexpr ← polyExpr poly
       let r ←
         if xn_ne:xn = 0 then
           let pr := mkAppN (mkConst ``mul_zero_lhs_poly_lemma) #[m, y, aexpr]
           -- aexpr + m*(0*y) = aexpr
-          pure (poly, pr)
+          pure { poly := poly, polyExpr := aexpr, equivProof := pr }
         else
           -- y_eq: aexpr + (m*x)*y = poly'.expr
-          let (poly, y_eq) ← appendAddExprFromInt (m * xn) (Int.mul_ne_zero m_ne xn_ne) y poly
-          let bexpr ← polyExpr poly
-          let pr := mkAppN (mkConst ``mul_lhs_poly_lemma) #[m, x, y, aexpr, bexpr]
-          pure (poly, pr)
+          let { poly := poly, polyExpr := bexpr, equivProof := y_pr }
+                ← appendAddExprFromInt (m * xn) (Int.mul_ne_zero m_ne xn_ne) y poly
+          let pr := mkAppN (mkConst ``mul_lhs_poly_lemma) #[m, x, y, aexpr, bexpr, y_pr]
+          pure { poly := poly, polyExpr := bexpr, equivProof := pr }
       return r
     -- Match second term is int literal.
     match ← matchIntLit y with
     | none => pure ()
     | some yn =>
-      let aexpr ← polyExpr poly
       let r ←
         if n_ne:yn = 0 then
           let pr := mkAppN (mkConst ``mul_zero_rhs_poly_lemma) #[m, x, aexpr]
-          pure (poly, pr)
+          pure { poly := poly, polyExpr := aexpr, equivProof := pr }
         else
-          let (p, x_eq) ← appendAddExprFromInt (m * yn) (Int.mul_ne_zero m_ne n_ne) x poly
-          let bexpr ← polyExpr poly
-          let pr := mkAppN (mkConst ``mul_rhs_poly_lemma) #[m, x, y, aexpr, bexpr]
-          pure (poly, pr)
+          let { poly := poly, polyExpr := bexpr, equivProof := x_pr }
+                ← appendAddExprFromInt (m * yn) (Int.mul_ne_zero m_ne n_ne) x poly
+          let { poly := poly, polyExpr := bexpr, equivProof := x_pr }
+                ← appendAddExprFromInt (m * yn) (Int.mul_ne_zero m_ne n_ne) x poly
+          let pr := mkAppN (mkConst ``mul_rhs_poly_lemma) #[m, x, y, aexpr, bexpr, x_pr]
+          pure { poly := poly, polyExpr := bexpr, equivProof := pr }
       return r
 
-  let v ← getUninterpVar (← instantiateMVars e)
-  let pr ← polyAddProof poly m m_ne v
-  pure (poly.add m v, pr)
+  let e ← instantiateMVars e
+  let (v, vExpr, eq) ← do
+        let r ← getVarForExpr e
+        pure (← getUninterpVar r.var, r.varExpr, r.eq)
+  let pr ← getPolyAddProof poly m m_ne v
+  let poly := poly.add m v
+  let bexpr ← getPolyExpr poly
+  let pr := mkAppN (mkConst ``uninterpVarLemma) #[e, vExpr, aexpr, m, bexpr, eq, pr]
+  pure { poly := poly, polyExpr := bexpr, equivProof := pr }
 
 theorem purifyIntLemmaPoly {x y:Int} (p:0 + 1 * x = y) : x = y := by
   simp [Int.zero_add, Int.one_mul] at p
@@ -269,22 +293,145 @@ theorem purifyIntLemmaVar {x y:Int} (p:0 + 1 * x = 1 * y) : x = y :=
 -- | This traverses an expression (which should have type int) to normalize
 -- the expression.  It produces a variable along with a proof that
 -- e = v.expr
-def purifyIntExpr (e:Expr) : ArithM (Var × Expr) := do
+def purifyIntExpr (e:Expr) : ArithM (ExprEvalResult TheoryVar) := do
   let e ← instantiateMVars e
-  have one_ne : (1:Int) ≠ 0 := by simp only [ne_eq]
-  let (p,pr) ← appendAddExprFromInt 1 one_ne e Poly.zero
+  let one_ne : (1:Int) ≠ 0 := by simp only [ne_eq]
+  let r ← appendAddExprFromInt 1 one_ne e Poly.zero
   -- pr  has type" 0 + 1 * e = p.expr"
-  match p with
+--  let { poly := p, polyExpr := pexpr := equivProof := pr} := r
+
+  match r.poly with
   | ⟨#[(1, v)]⟩ => do
     -- Make pr have type e = v
-    let pr := mkAppN (mkConst ``purifyIntLemmaVar) #[e, ← varExpr v, pr]
-    pure (v, pr)
-  | otherwise => do
+    let ve ← getThvarExpr v
+    let pr := mkAppN (mkConst ``purifyIntLemmaVar) #[e, ve, r.equivProof]
+    pure {var := v, varExpr := ve, eq := r.equivProof }
+  | p => do
     let v ← getPolyVar p
     -- Make pr have type e = v
-    let pr := mkAppN (mkConst ``purifyIntLemmaPoly) #[e, ← polyExpr p, pr]
-    pure (v, pr)
+    let pr := mkAppN (mkConst ``purifyIntLemmaPoly) #[e, r.polyExpr, r.equivProof]
+    pure {var := v, varExpr := r.polyExpr, eq := pr }
 
 end Normalization
 
+def ops (r:IO.Ref State) : TheoryOps :=
+  { varExpr := mthvarExpr r,
+    predExpr := ArithTheory.predExpr r
+    exprVar := fun e => purifyIntExpr e r
+  }
+
+section PredicateNormalizationLemmas
+
+theorem nat_lt_prop {x y : Nat} (p : x < y)
+  : Int.NonNeg (OfNat.ofNat y - OfNat.ofNat (x + 1)) := Int.nonNeg_of_nat_le p
+def nat_ge_prop {x y : Nat} (p : x ≥ y) := Int.nonNeg_of_nat_le p
+def nat_gt_prop {x y : Nat} (p : x > y) := Int.nonNeg_of_nat_le p
+
+theorem nat_not_le_prop {x y : Nat} (p : ¬(x ≤ y)) : Int.NonNeg (OfNat.ofNat x - OfNat.ofNat (y + 1)) :=
+  match Nat.lt_or_ge y x with
+  | Or.inl q => Int.nonNeg_of_nat_le q
+  | Or.inr q => False.elim (p q)
+theorem nat_not_lt_prop {x y : Nat} (p : ¬(x < y))
+  : Int.NonNeg (OfNat.ofNat x - OfNat.ofNat y) :=
+  match Nat.lt_or_ge x y with
+  | Or.inl q => False.elim (p q)
+  | Or.inr q => Int.nonNeg_of_nat_le q
+def nat_not_ge_prop {x y : Nat} (p : ¬(x ≥ y)) := nat_not_le_prop p
+def nat_not_gt_prop {x y : Nat} (p : ¬(x > y)) := nat_not_lt_prop p
+
+theorem int_le_prop {x y : Int} (p : x ≤ y) : Int.NonNeg (y - x) := p
+theorem int_lt_prop {x y : Int} (p : x < y) : Int.NonNeg (y - (x + 1)) := p
+def int_ge_prop {x y : Int} (p : x ≥ y) := int_le_prop p
+def int_gt_prop {x y : Int} (p : x > y) := int_lt_prop p
+
+theorem int_not_le_prop {x y : Int} (p : ¬(x ≤ y))
+  : Int.NonNeg (x - (y + 1)) :=
+  match Int.lt_or_ge y x with
+  | Or.inl q => int_lt_prop q
+  | Or.inr q => False.elim (p q)
+
+theorem int_not_lt_prop {x y : Int} (p : ¬(x < y))
+  : Int.NonNeg (x - y) :=
+  match Int.lt_or_ge x y with
+  | Or.inl q => False.elim (p q)
+  | Or.inr q => int_le_prop q
+def int_not_ge_prop {x y : Int} (p : ¬(x ≥ y)) := int_not_le_prop p
+def int_not_gt_prop {x y : Int} (p : ¬(x > y)) := int_not_lt_prop p
+
+theorem int_eq_prop (x y : Int) (p : x = y)
+  : x - y = 0 := by simp [p, Int.sub_self]
+
+theorem nat_eq_prop {x y : Nat} (p : x = y)
+  : @OfNat.ofNat Int x _ - OfNat.ofNat y = 0 := by
+    apply int_eq_prop
+    simp only [OfNat.ofNat, p]
+
+theorem int_not_eq_prop {x y : Int} (p : ¬(x = y))  : ¬(x - y = 0) := by
+  intro q
+  apply p (Int.sub_eq_zero_implies_eq q)
+
+theorem nat_not_eq_prop {x y : Nat} (p : ¬(x = y))
+  : ¬(@OfNat.ofNat Int x _ - OfNat.ofNat y = 0) := by
+  apply int_not_eq_prop
+  simp only [OfNat.ofNat, Int.ofNat.injEq]
+  exact p
+
+def transformerNames : Array Name :=
+  #[
+    ``nat_eq_prop,
+    ``nat_lt_prop,
+    ``Int.nonNeg_of_nat_le,
+    ``nat_gt_prop,
+    ``nat_ge_prop,
+    ``nat_not_eq_prop,
+    ``nat_not_lt_prop,
+    ``nat_not_le_prop,
+    ``nat_not_gt_prop,
+    ``nat_not_ge_prop,
+    ``int_eq_prop,
+    ``int_lt_prop,
+    ``int_le_prop,
+    ``int_gt_prop,
+    ``int_ge_prop,
+    ``int_not_eq_prop,
+    ``int_not_lt_prop,
+    ``int_not_le_prop,
+    ``int_not_gt_prop,
+    ``int_not_ge_prop
+  ]
+
+end PredicateNormalizationLemmas
+
+-- Lemma used for convert proofs from one type of predicate to another.
+private theorem intNonNeg_lemma {x y :Int} (eq:x = y) (p:Int.NonNeg x) : Int.NonNeg y := eq.subst p
+private theorem intEq0_lemma {x y :Int} (eq:x = y) (p:x = 0) : y = 0 := @Eq.subst Int (λd => d = 0) _ _ eq p
+private theorem intNe0_lemma {x y :Int} (eq:x = y) (p:¬(x = 0)) : ¬(y = 0) := @Eq.subst Int (λd => ¬(d = 0)) _ _ eq p
+
+-- | Match `(Int.NonNeg e) and return proof term and property.
+def matchIntNonNeg (r:IO.Ref ArithTheory.State)  (prop : Expr) : SolverM (Option (TheoryPred × Expr)) := do
+  let mvar ← mkFreshExprMVar intExpr MetavarKind.natural `n
+  unless ← isDefEq (mkIntNonNegExpr mvar) prop do
+    return none
+  let res ← purifyIntExpr mvar r
+  let pred ← getTheoryPred (Pred.IsGe0 res.var) r
+  let proofFn := mkAppN (mkConst ``intNonNeg_lemma) #[mvar, ← getThvarExpr res.var r, res.eq]
+  return (some (pred, proofFn))
+
+def matchIntEq0 (r:IO.Ref ArithTheory.State) (prop : Expr) : SolverM (Option (TheoryPred × Expr)) := do
+  let mvar ← mkFreshExprMVar intExpr MetavarKind.natural `n
+  unless ← isDefEq (mkIntEq0Expr mvar) prop do
+    return none
+  let res ← purifyIntExpr mvar r
+  let proofFn := mkAppN (mkConst ``intEq0_lemma) #[mvar, ← getThvarExpr res.var r, res.eq]
+  return (some (← getTheoryPred (Pred.IsEq0 res.var) r, proofFn))
+
+def matchNotIntEq0 (r:IO.Ref ArithTheory.State) (prop : Expr) : SolverM (Option (TheoryPred × Expr)) := do
+  let mvar ← mkFreshExprMVar intExpr MetavarKind.natural `n
+  unless ← isDefEq (mkApp (mkConst ``Not) (mkIntEq0Expr mvar)) prop do
+    return none
+  let res ← purifyIntExpr mvar r
+  let proofFn := mkAppN (mkConst ``intNe0_lemma) #[mvar, ← getThvarExpr res.var r, res.eq]
+  return (some (← getTheoryPred (Pred.IsNe0 res.var) r, proofFn))
+
+end ArithTheory
 end ArithSolver
