lib/ArithSolver/Tests.lean
@@ -10,7 +10,6 @@ structure Hide (P:Prop) := { value : P }
 def test_false_goal (p:Hide False) : False := by
   to_poly
   exact p.value
-
 def test_uninterp_goal (p:Hide False) : Hide True := by
   to_poly
   exact p.value
@@ -20,15 +19,16 @@ def test_uninterp_goal (p:Hide False) : Hide True := by
 --  to_poly
 --  exact p.value negGoal
 
+
 theorem test_le_int_goal (x y:Int) (p:Hide (¬Int.NonNeg (-1 + -1 * y))) : x ≤ x + y := by
   to_poly
   exact p.value negGoal
 
-def test_eq_goal (x:Int) (p : Hide (-1 * y + 1 * x = 0)) : x = y := by
+def test_eq_goal (x:Int) (p : Hide (1 * x + -1 * y = 0)) : x = y := by
   to_poly
   exact (negGoal p.value)
 
-def test_ne_goal (x:Int) (p : Hide (¬(-y + x = 0))) : x ≠ y := by
+def test_ne_goal (x:Int) (p : Hide (¬(x + -y = 0))) : x ≠ y := by
   to_poly
   simp only [Int.one_mul, Int.neg_one_mul] at negGoal
   exact p.value negGoal
@@ -42,7 +42,9 @@ def test_ground_assumption (q:1 + 2 = 4): False := by
   contradiction
 
 /- TODO: Exlore additional test cases
-def test_not_goal (a b : Nat) : ¬(a > b) := by
+def test_not_goal (a b : Nat)
+     (p:Hide (Int.NonNeg (1 * OfNat.ofNat a + -1 * OfNat.ofNat (b + 1))))
+     : ¬(a > b) := by
   to_poly
 
 def test_nat_gt_goal (a b : Nat) : (a > b) := by
