lib/ArithSolver/ToPoly.lean
@@ -3,6 +3,7 @@ This module defines operations for constructing a
 linear arithmetic state form a Lean context while
 ensuring Lean proofs can be constructed from SAT check.
 -/
+import ArithSolver.ConstantTheory
 import ArithSolver.IntNormalization
 import Lean
 
@@ -12,21 +13,153 @@ open Lean.Elab.Tactic
 
 namespace ArithSolver
 
-private def ofNatExpr : Expr := mkConst ``Int.ofNat
-private def intNonNegMkExpr : Expr := mkConst ``Int.NonNeg.mk
+section ExpressionUtils
+
 private def propExpr : Expr := mkSort levelZero
 
 def falseExpr : Expr := mkConst ``False
+
+def exprHead : Expr → Option Name
+| Expr.bvar .. => none
+-- FIXME: Figure out if we want to see through free variables with let bindings in local context.
+| Expr.fvar .. => none
+| Expr.mvar .. => none
+| Expr.sort .. => none
+| Expr.const nm .. => nm
+| Expr.app f a .. => exprHead f
+| Expr.lam .. => none
+| Expr.forallE .. => none
+-- FIXME: Figure out if we want to see through let bindings.
+| Expr.letE .. => none
+| Expr.lit .. =>  none
+-- FIXME: Figure out if ignoring metadata is always ok.
+| Expr.mdata  _ x .. => exprHead x
+ -- FIXME: Figure out if we want to see through projections.
+| Expr.proj n i s .. => none
+
+end ExpressionUtils
+
+-- | Assertion added
+structure Assertion where
+  -- Identifies the free variable in the initial context used to generate this one.
+  -- Used to allow deleting original proposition from local context.
+  origin : Option FVarId
+  -- The free variable used to identify the assertion in the local context
+  -- generated for the assertion.
+  name : Name
+  -- A proof of the assertion in the context of the original goal.
+  proof : Expr
+  -- Predicate that was asserted.
+  pred : Pred
+
+namespace Assertion
+
+instance : Inhabited Assertion := ⟨
+     { origin := arbitrary,
+       name := arbitrary,
+       proof := arbitrary,
+       pred := arbitrary
+     }
+  ⟩
+
+end Assertion
+
+def uninterpTheoryRef : TheoryRef := ⟨0⟩
+
+structure Context where
+  -- Maps constant names to the theory associated with that constant.
+  constTheoryMap : Std.PersistentHashMap Name TheoryRef
+  -- An array of theory operation.
+  -- The first theory is used for uninterpreted constants.
+  theories : Array TheoryOps
+
+namespace Context
+
+partial def varExpr (ctx:Context) (v:Var) : IO Expr := do
+  let th := ctx.theories[v.theory.toNat]
+  th.varExpr (varExpr ctx) v.theoryVar
+
+def predExpr (ctx:Context) (p:Pred) : IO Expr := do
+  let ref := p.theory.toNat
+  if h : ref < ctx.theories.size then
+    let ops := (ctx.theories.get ⟨ref, h⟩)
+    let e ← ops.predExpr (ctx.varExpr) p.theoryPred
+    pure e
+  else
+    panic! "Invalid theory index."
+
+mutual
+
+-- | Create a variable for the current expression from a theory.
+--
+-- The source theory is the theory that initiated the request from a variable.
+-- If the expression head is assigned to this theory, then we ensure this is an
+-- uninterpreted symbol.
+partial
+def exprVar (ctx:Context) (e:Expr) : MetaM (ExprEvalResult Var) := do
+  -- Get theory associated with head symbol.
+  let mut thRef :=
+        match exprHead e with
+        | some head => ctx.constTheoryMap.findD head uninterpTheoryRef
+        | none => uninterpTheoryRef
+  let th := ctx.theories[thRef.toNat]
+  let r ← th.exprVar e (services ctx)
+  pure { r with var := Var.mkVar thRef r.var }
+
+partial
+def services (ctx:Context) : SolverServices := {
+    varExpr := varExpr ctx,
+    uninterpVar := fun e => do
+      let thRef := uninterpTheoryRef
+      let th := ctx.theories[thRef.toNat]
+      let r ← th.exprVar e (services ctx)
+      pure (Var.mkVar thRef r.var)
+    exprVar := exprVar ctx,
+  }
+
+end
+
+end Context
+
+structure State where
+  -- Predicates asserted to be true.
+  assertions : Array Assertion := #[]
+
+namespace State
+
+
+-- | Return proofs associated with assertions.
+def proofs (s:State) : Array Expr := s.assertions.map Assertion.proof
+
+-- | Add assertions to local context.
+-- Return new local context along with array of free variables identifying assertions.
+def addAssertions (ctx:Context) (s:State) (lctx:LocalContext) : MetaM (LocalContext × Array Expr) := do
+  let mut lctx := lctx
+  let mut fvars : Array Expr := #[]
+  for a in s.assertions do
+    let newVar ← mkFreshFVarId
+    fvars := fvars.push (mkFVar newVar)
+    match a.origin with
+    | some prevVar =>
+      -- FIXME: Make sure erasing the previous declaration does not break things.
+      lctx := lctx.erase prevVar
+    | none =>
+      pure ()
+    let e ← ctx.predExpr a.pred
+    lctx := lctx.mkLocalDecl newVar a.name e
+  pure (lctx, fvars)
+
+end State
 
 structure Goal where
   -- Given a proof from the solver
   onMkProof : Expr → Expr
 
-def Goal.onAddAssumptions (tactic:Name) (g:Goal) (goalId:MVarId) (s:State) : MetaM (List MVarId) := do
+def Goal.onAddAssumptions (ctx:Context) (tactic:Name) (g:Goal) (goalId:MVarId) (s:State) : MetaM (List MVarId) := do
   checkNotAssigned goalId tactic
   let tag   ← getMVarTag goalId
   let lctx ← getLCtx
-  let (lctx, fvars) ← s.addAssertions lctx
+  let (lctx, fvars) ← State.addAssertions ctx s lctx
   withReader (fun ctx => { ctx with lctx := lctx }) $ do
     let solverGoal ← mkFreshExprSyntheticOpaqueMVar falseExpr tag
     -- Turn goal into lambda with free variables from assertions
@@ -78,165 +211,54 @@ def resolveTransformerArgs (proofExpr:Expr) (t:Transformer) : MetaM Bool := do
       throwError m!"Unresolved transformer argument in {indentExpr proofExpr}"
   return true
 
--- | Match `(Int.NonNeg e) and return e
-def matchIntNonNeg (e:Expr) : MetaM (Option Expr) := do
-  let mvar ← mkFreshExprMVar intExpr MetavarKind.natural `n
-  pure $ if ← isDefEq (mkIntNonNegExpr mvar) e then some mvar else none
+-- | A rule that given a proposition, tries to produce a predicate
+-- and a function expression that transforms proofs of the original
+-- proposition into proofs of the predicate.
+structure PredRule where
+  theoryRef : TheoryRef
+  action (prop : Expr) : SolverM (Option (TheoryPred × Expr))
 
-def matchIntEq0 (e:Expr) : MetaM (Option Expr) := do
-  let mvar ← mkFreshExprMVar intExpr MetavarKind.natural `n
-  pure $ if ← isDefEq (mkIntEq0Expr mvar) e then some mvar else none
-
-def matchNotIntEq0 (e:Expr) : MetaM (Option Expr) := do
-  let mvar ← mkFreshExprMVar intExpr MetavarKind.natural `n
-  if ← isDefEq (mkApp (mkConst ``Not) (mkIntEq0Expr mvar)) e then
-    pure $ some mvar
-  else
-    none
-
-def matchNot (e:Expr) : MetaM (Option Expr) := do
-  let mvar ← mkFreshExprMVar propExpr MetavarKind.natural `a
-  let p := mkApp (mkConst ``Not) mvar
-  pure $ if ← isDefEq p e then mvar else none
-
-section PredicateNormalizationLemmas
-
-theorem nat_lt_prop {x y : Nat} (p : x < y)
-  : Int.NonNeg (OfNat.ofNat y - OfNat.ofNat (x + 1)) := Int.nonNeg_of_nat_le p
-def nat_ge_prop {x y : Nat} (p : x ≥ y) := Int.nonNeg_of_nat_le p
-def nat_gt_prop {x y : Nat} (p : x > y) := Int.nonNeg_of_nat_le p
-
-theorem nat_not_le_prop {x y : Nat} (p : ¬(x ≤ y)) : Int.NonNeg (OfNat.ofNat x - OfNat.ofNat (y + 1)) :=
-  match Nat.lt_or_ge y x with
-  | Or.inl q => Int.nonNeg_of_nat_le q
-  | Or.inr q => False.elim (p q)
-theorem nat_not_lt_prop {x y : Nat} (p : ¬(x < y))
-  : Int.NonNeg (OfNat.ofNat x - OfNat.ofNat y) :=
-  match Nat.lt_or_ge x y with
-  | Or.inl q => False.elim (p q)
-  | Or.inr q => Int.nonNeg_of_nat_le q
-def nat_not_ge_prop {x y : Nat} (p : ¬(x ≥ y)) := nat_not_le_prop p
-def nat_not_gt_prop {x y : Nat} (p : ¬(x > y)) := nat_not_lt_prop p
-
-theorem int_le_prop {x y : Int} (p : x ≤ y) : Int.NonNeg (y - x) := p
-theorem int_lt_prop {x y : Int} (p : x < y) : Int.NonNeg (y - (x + 1)) := p
-def int_ge_prop {x y : Int} (p : x ≥ y) := int_le_prop p
-def int_gt_prop {x y : Int} (p : x > y) := int_lt_prop p
-
-theorem int_not_le_prop {x y : Int} (p : ¬(x ≤ y))
-  : Int.NonNeg (x - (y + 1)) :=
-  match Int.lt_or_ge y x with
-  | Or.inl q => int_lt_prop q
-  | Or.inr q => False.elim (p q)
-
-theorem int_not_lt_prop {x y : Int} (p : ¬(x < y))
-  : Int.NonNeg (x - y) :=
-  match Int.lt_or_ge x y with
-  | Or.inl q => False.elim (p q)
-  | Or.inr q => int_le_prop q
-def int_not_ge_prop {x y : Int} (p : ¬(x ≥ y)) := int_not_le_prop p
-def int_not_gt_prop {x y : Int} (p : ¬(x > y)) := int_not_lt_prop p
-
-theorem int_eq_prop (x y : Int) (p : x = y)
-  : x - y = 0 := by simp [p, Int.sub_self]
-
-theorem nat_eq_prop {x y : Nat} (p : x = y)
-  : @OfNat.ofNat Int x _ - OfNat.ofNat y = 0 := by
-    apply int_eq_prop
-    simp only [OfNat.ofNat, p]
-
-theorem int_not_eq_prop {x y : Int} (p : ¬(x = y))  : ¬(x - y = 0) := by
-  intro q
-  apply p (Int.sub_eq_zero_implies_eq q)
-
-theorem nat_not_eq_prop {x y : Nat} (p : ¬(x = y))
-  : ¬(@OfNat.ofNat Int x _ - OfNat.ofNat y = 0) := by
-  apply int_not_eq_prop
-  simp only [OfNat.ofNat, Int.ofNat.injEq]
-  exact p
-
-end PredicateNormalizationLemmas
-
--- Lemma used for convert proofs from one type of predicate to another.
-private theorem intNonNeg_lemma {x y :Int} (eq:x = y) (p:Int.NonNeg x) : Int.NonNeg y := eq.subst p
-private theorem intEq0_lemma {x y :Int} (eq:x = y) (p:x = 0) : y = 0 := @Eq.subst Int (λd => d = 0) _ _ eq p
-private theorem intNe0_lemma {x y :Int} (eq:x = y) (p:¬(x = 0)) : ¬(y = 0) := @Eq.subst Int (λd => ¬(d = 0)) _ _ eq p
-
--- | Analyze a proof and a proposition to produce a Linear arith predicate along with a proof
--- that of the predicate.
-partial def extractPropPred (proof:Expr) (prop:Expr) : ArithM (Option (Expr × Pred)) := do
-  -- Check if prop matches (Int.NonNeg e)
-  match ← matchIntNonNeg prop with
-  | none => pure ()
-  | some e =>
-    let (v, pr) ← purifyIntExpr e
-    let proof := mkAppN (mkConst ``intNonNeg_lemma) #[e, ← varExpr v, pr, proof]
-    return (some (proof, Pred.IsGe0 v))
-  -- Check if prop match (e = Int.ofNat 0)
-  match ← matchIntEq0 prop with
-  | none => pure ()
-  | some e =>
-    let (v, pr) ← purifyIntExpr e
-    let proof := mkAppN (mkConst ``intEq0_lemma) #[e, ← varExpr v, pr, proof]
-    return (some (proof, Pred.IsEq0 v))
-  match ← matchNotIntEq0 prop with
-  | none => pure ()
-  | some e =>
-    let (v, pr) ← purifyIntExpr e
-    let proof := mkAppN (mkConst ``intNe0_lemma) #[e, ← varExpr v, pr, proof]
-    return (some (proof, Pred.IsNe0 v))
-  let mkTrans (nm:Name) : Expr := mkConst nm
-  -- Create list of transformers to apply
-  let transformers : Array Expr := #[
-          mkTrans ``nat_eq_prop,
-          mkTrans ``nat_lt_prop,
-          mkTrans ``Int.nonNeg_of_nat_le,
-          mkTrans ``nat_gt_prop,
-          mkTrans ``nat_ge_prop,
-          mkTrans ``nat_not_eq_prop,
-          mkTrans ``nat_not_lt_prop,
-          mkTrans ``nat_not_le_prop,
-          mkTrans ``nat_not_gt_prop,
-          mkTrans ``nat_not_ge_prop,
-          mkTrans ``int_eq_prop,
-          mkTrans ``int_lt_prop,
-          mkTrans ``int_le_prop,
-          mkTrans ``int_gt_prop,
-          mkTrans ``int_ge_prop,
-          mkTrans ``int_not_eq_prop,
-          mkTrans ``int_not_lt_prop,
-          mkTrans ``int_not_le_prop,
-          mkTrans ``int_not_gt_prop,
-          mkTrans ``int_not_ge_prop
-        ]
-  let mut found : Option (Expr × Expr) := none
-  -- Iterate through list looking for first match
-  for rule in transformers do
-    -- Get variables and type of proof
-    let t ← mkTransformer rule
-    unless ← isDefEq t.assumptionType prop do
-      continue
-    unless ← resolveTransformerArgs rule t do
-      continue
-    found := (mkApp (mkAppN rule t.arguments) proof, t.resultType)
-    break
-  match found with
-  | none =>
-    pure none
-  | some (proof, prop) => do
-    extractPropPred proof prop
+def runTerminals (terminals:Array PredRule) (prop:Expr) : SolverM (Option (Pred × Expr)) := do
+  for t in terminals do
+    match ← t.action prop with
+    | none => pure ()
+    | some (p, transform) =>
+      return (some (Pred.mkPred t.theoryRef p, transform))
+  return none
 
 -- | See if we can add the local declaration to the arithmetic unit.
 -- proof is a term of type prop.
-def processAssumptionProp (origin : Option FVarId) (name:Name) (proof:Expr) (prop:Expr) : ArithM Bool := do
-  match ← extractPropPred proof prop with
+def addAssertion (prules:Array PredRule)
+                 (r:IO.Ref State)
+                 (origin : Option FVarId)
+                 (name:Name)
+                 (proof:Expr)
+                 (prop:Expr) : SolverM Bool := do
+  match ← runTerminals prules prop with
   | none => do
     pure false
-  | some (proof, pred) => do
-    assertPred origin name proof pred
+  | some (pred, proofFn) => do
+    let a := { origin := origin, name := name, proof := mkApp proofFn proof, pred := pred }
+    r.modify $ λs => { s with assertions := s.assertions.push a }
     pure true
 
-def processDecls (lctx:LocalContext) : ArithM Unit := do
+namespace ArithTheory
+
+private def intNonNegMkExpr : Expr := mkConst ``Int.NonNeg.mk
+private def ofNatExpr : Expr := mkConst ``Int.ofNat
+
+def matchNatExpr (prules:Array PredRule) (r:IO.Ref ArithSolver.State) (nm:Name) (e:Expr) (tp:Expr) : SolverM Bool := do
+  unless (← isDefEq tp natExpr) do
+    return false
+  -- Assert v is non negative
+  let proof := mkApp intNonNegMkExpr e
+  let prop := mkIntNonNegExpr (mkApp ofNatExpr e)
+  _ ← addAssertion prules r none (nm ++ "isGe0") proof prop
+  return true
+
+end ArithTheory
+
+def processDecls (prules:Array PredRule) (r:IO.Ref State) (lctx:LocalContext) : SolverM Unit := do
   let mut seenFirst := false
   for md in lctx.decls do
     -- Skip first declaration (as it corresponds to initial goal for
@@ -247,23 +269,15 @@ def processDecls (lctx:LocalContext) : ArithM Unit := do
     -- Skip if declaration has been deleted.
     let some d ← pure md
          | continue
-    -- TODO: Figure out how to support let declarations
+    -- FIXME: Figure out how to support let declarations
     if d.isLet then
       continue
     -- If we have a natural number, then declare it.
-    if ← isDefEq d.type natExpr then
-      let v ← getUninterpVar (mkApp ofNatExpr (mkFVar d.fvarId))
-      -- Assert v is non negative
-      let proof := mkApp intNonNegMkExpr (mkFVar d.fvarId)
-      assertPred none (d.userName ++ "isGe0") proof (Pred.IsGe0 v)
-      continue
-    -- If we have a natural number, then declare it.
-    if ← isDefEq d.type intExpr then
-      let v ← getUninterpVar (mkFVar d.fvarId)
+    if ← ArithTheory.matchNatExpr prules r d.userName (mkFVar d.fvarId) d.type then
       continue
     -- If this is a proposition then try assuming it.
     if ← isDefEq (← inferType d.type) propExpr then do
-      let _ ← processAssumptionProp (some d.fvarId) d.userName (mkFVar d.fvarId) d.type
+      let _ ← addAssertion prules r (some d.fvarId) d.userName (mkFVar d.fvarId) d.type
 
 -- Negating goal
 
@@ -272,7 +286,12 @@ theorem decidable_by_contra {P:Prop} [h:Decidable P] (q : ¬¬P) : P :=
   | isFalse h => False.elim (q h)
   | isTrue h => h
 
-def analyzeGoal (tactic:Name) (goalId:MVarId) (target:Expr) : ArithM Goal := do
+def matchNot (e:Expr) : MetaM (Option Expr) := do
+  let mvar ← mkFreshExprMVar propExpr MetavarKind.natural `a
+  let p := mkApp (mkConst ``Not) mvar
+  pure $ if ← isDefEq p e then mvar else none
+
+def analyzeGoal (prules:Array PredRule) (r : IO.Ref State) (tactic:Name) (goalId:MVarId) (target:Expr) : SolverM Goal := do
   -- If goal is already false, then just negate it.
   if ← isDefEq target falseExpr then
     return { onMkProof := id }
@@ -280,14 +299,14 @@ def analyzeGoal (tactic:Name) (goalId:MVarId) (target:Expr) : ArithM Goal := do
   -- If goal has form `Not p` then we can diretly process property.
   match ← matchNot target with
   | some prop => do
-    if ← processAssumptionProp none `negGoal (mkBVar 0) prop then
+    if ← addAssertion prules r none `negGoal (mkBVar 0) prop then
       return { onMkProof := mkLambda Name.anonymous BinderInfo.default prop }
   -- Goal is not a negation, so we seeing if we can extract a predicate from
   -- negated goal and then use decidable_by_contra to get proof of negation
   -- of target.
   | none =>
     let prop := mkApp (mkConst ``Not) target
-    if ← processAssumptionProp none `negGoal (mkBVar 0) prop then
+    if ← addAssertion prules r none `negGoal (mkBVar 0) prop then
       let some classVal ← synthInstance? (mkApp (mkConst ``Decidable) target)
           | throwTacticEx tactic goalId "Could not synthesize Decidable instance for proposition:."
       let decideByContraExpr := mkAppN (mkConst ``decidable_by_contra) #[target, classVal]
@@ -306,18 +325,74 @@ def analyzeGoal (tactic:Name) (goalId:MVarId) (target:Expr) : ArithM Goal := do
   | _ =>
     throwTacticEx tactic goalId "Expected a type."
 
-def mkArithGoal (tactic:Name) (goalId:MVarId) : MetaM (Goal × State) := ArithM.run do
+def mkTermTrans (thref:TheoryRef) (terminals:Array PredRule) (nm:Name) : PredRule :=
+  { theoryRef := thref,
+    action := fun (prop:Expr) => do
+      let rule := mkConst nm
+      let trans ← mkTransformer rule
+      unless ← isDefEq trans.assumptionType prop do
+        return none
+      unless ← resolveTransformerArgs rule trans do
+        return none
+      let propProofFn := mkAppN rule trans.arguments
+      for t in terminals do
+        match ← t.action trans.resultType with
+        | none =>
+          pure ()
+        | some (pred, nextProofFn) => do
+          let finalProofFn :=
+                mkLambda Name.anonymous BinderInfo.default prop
+                  (mkApp nextProofFn (mkApp propProofFn (mkBVar 0)))
+          return (some (pred, finalProofFn))
+      return none
+  }
+
+def mapFromList (l:List (Name × TheoryRef)) : Std.PersistentHashMap Name TheoryRef := Id.run do
+  let mut r := {}
+  for (nm,ref) in l do
+    r := r.insert nm ref
+  pure r
+
+abbrev arithTheoryRef : TheoryRef := ⟨1⟩
+
+def mkArithGoal (terminals: Array PredRule) (tactic:Name) (goalId:MVarId) : SolverM (Goal × State) := do
   withMVarContext goalId do
     let md ← getMVarDecl goalId
-    processDecls md.lctx
-    analyzeGoal tactic goalId md.type
+    let stateRef ← IO.mkRef {}
+    processDecls terminals stateRef md.lctx
+    let g ← analyzeGoal terminals stateRef tactic goalId md.type
+    pure (g, ← stateRef.get)
 
 syntax (name := to_poly) "to_poly" : tactic
 
 @[tactic to_poly] def evalToPoly : Tactic := fun stx => do
   liftMetaTactic fun mvarId => do
-    let (goal, s) ← mkArithGoal `to_poly mvarId
-    let r@([goalId]) ← goal.onAddAssumptions `to_poly mvarId s
+    let constRef ← IO.mkRef {}
+    let arithRef ← IO.mkRef {}
+    let ctx : Context := {
+      constTheoryMap := mapFromList [
+        (``HAdd.hAdd, arithTheoryRef),
+        (``HSub.hSub, arithTheoryRef),
+        (``HMul.hMul, arithTheoryRef)
+      ],
+      theories := #[ConstantTheory.ops constRef, ArithTheory.ops arithRef ]
+    }
+    let terminals := #[
+            ArithTheory.matchIntNonNeg arithRef,
+            ArithTheory.matchIntEq0 arithRef,
+            ArithTheory.matchNotIntEq0 arithRef
+          ]
+    let convTerm (f : Expr → SolverM (Option (TheoryPred × Expr))) : PredRule :=
+          { theoryRef := arithTheoryRef,
+            action := f
+          }
+    let terminals := terminals.map convTerm
+    -- Create list of transformers to apply
+    let transformers := ArithTheory.transformerNames.map (mkTermTrans arithTheoryRef terminals)
+    let terminals := terminals ++ transformers
+
+    let (goal, s) ← mkArithGoal terminals `to_poly mvarId ctx.services
+    let r@([goalId]) ← goal.onAddAssumptions ctx `to_poly mvarId s
       | throwError "Expected more goals"
     pure r
 
